theories/HoareDef.v
@@ -3,7 +3,6 @@ Require Import Universe.
 Require Import STS.
 Require Import Behavior.
 Require Import ModSem.
-Import EventsL ModSemL.
 Require Import Skeleton.
 Require Import PCM.
 From Ordinal Require Export Ordinal Arithmetic Inaccessible.
